theories/lang/lang.v
@@ -1,256 +1,304 @@
 From iris.program_logic Require Export language ectx_language ectxi_language.
 From stdpp Require Export strings.
 From stdpp Require Import gmap list.
-From refinedc.lang Require Export base.
+From refinedc.lang Require Export base byte layout int_type.
 Set Default Proof Using "Type".
 
 Open Scope Z_scope.
 
-(** Representation of a standard (8-bit) byte. *)
-Section Byte.
-  Definition bits_per_byte : Z := 8.
-
-  Definition byte_modulus : Z :=
-    Eval cbv in 2 ^ bits_per_byte.
-
-  Record byte :=
-    Byte {
-      byte_val : Z;
-      byte_constr : -1 < byte_val < byte_modulus;
-    }.
-
-  Global Instance byte_eq_dec : EqDecision byte.
-  Proof.
-    move => [b1 H1] [b2 H2]. destruct (decide (b1 = b2)) as [->|].
-    - left. assert (H1 = H2) as ->; [|done]. apply proof_irrel.
-    - right. naive_solver.
-  Qed.
-
-  Program Definition byte0 : byte := {|
-    byte_val := 0;
-  |}.
-  Next Obligation. done. Qed.
-End Byte.
-
-(** Representation of a type layout (byte size and alignment constraint). *)
-Section Layout.
-  Record layout :=
-    Layout {
-      ly_size : nat;
-      ly_align_log : nat;
-    }.
-
-  Definition sizeof   (ly : layout) : nat := ly.(ly_size).
-  Definition ly_align (ly : layout) : nat := 2 ^ ly.(ly_align_log).
-
-  Global Instance layout_dec_eq : EqDecision layout.
-  Proof. solve_decision. Defined.
-
-  Global Instance layout_inhabited : Inhabited layout :=
-    populate (Layout 0 0).
-
-  Global Instance layout_countable : Countable layout.
-  Proof.
-    refine (inj_countable'
-      (λ ly, (ly.(ly_size), ly.(ly_align_log)))
-      (λ '(sz, a), Layout sz a) _); by intros [].
-  Qed.
-
-  Global Instance layout_le : SqSubsetEq layout := λ ly1 ly2,
-    (ly1.(ly_size) ≤ ly2.(ly_size))%nat ∧
-    (ly1.(ly_align_log) ≤ ly2.(ly_align_log))%nat.
-
-  Global Instance layout_le_po : PreOrder layout_le.
-  Proof.
-    split => ?; rewrite /layout_le => *; repeat case_bool_decide => //; lia.
-  Qed.
-
-  Definition ly_offset (ly : layout) (n : nat) : layout := {|
-    ly_size := ly.(ly_size) - n;
-    (* Sadly we need to have the second argument to factor2 as we want
-    that if l is aligned to x, then l + n * x is aligned to x for all n
-    including 0. *)
-    ly_align_log := ly.(ly_align_log) `min` factor2 n ly.(ly_align_log)
-  |}.
-
-  Definition ly_set_size (ly : layout) (n : nat) : layout := {|
-    ly_size := n;
-    ly_align_log := ly.(ly_align_log)
-  |}.
-
-  Definition ly_mult (ly : layout) (n : nat) : layout := {|
-    ly_size := ly.(ly_size) * n;
-    ly_align_log := ly.(ly_align_log)
-  |}.
-
-  Definition ly_with_align (sz : nat) (align : nat) : layout := {|
-    ly_size := sz;
-    ly_align_log := factor2 align 0
-  |}.
-
-  Definition layout_wf (ly : layout) : Prop := (ly_align ly | ly.(ly_size)).
-
-  Lemma layout_wf_mod (ly : layout) :
-    ly.(ly_size) `mod` ly_align ly = 0 → layout_wf ly.
-  Proof.
-    move => ?. apply Z.mod_divide => //. have ->: 0 = O by [].
-    move => /Nat2Z.inj/Nat.pow_nonzero. lia.
-  Qed.
-
-  Class LayoutWf (ly : layout) : Prop := layout_wf_wf : layout_wf ly.
-
-  (* Class required because the combinators of layout are made typeclass opaque
-     later, so TCEq does not work. *)
-  Class LayoutEq (ly1 ly2 : layout) : Prop := layout_eq : ly1 = ly2.
-End Layout.
-
-Arguments ly_size : simpl never.
-Arguments sizeof _ /.
-(*Arguments ly_align_log : simpl never.*)
-Arguments ly_align : simpl never.
-
-Typeclasses Opaque layout_le ly_offset ly_set_size ly_mult ly_with_align.
-
-Hint Extern 0 (LayoutWf _) => refine (layout_wf_mod _ _); done : typeclass_instances.
-Hint Extern 0 (LayoutWf _) => unfold LayoutWf; done : typeclass_instances.
-Hint Extern 0 (LayoutEq _ _) => exact: eq_refl : typeclass_instances.
-
-(** Representation of an integer type (size and signedness). *)
-Section IntType.
-  Definition signed := bool.
-
-  Record int_type :=
-    IntType {
-      it_byte_size_log : nat;
-      it_signed : signed;
-    }.
-
-  Definition bytes_per_int (it : int_type) : nat :=
-    2 ^ it.(it_byte_size_log).
-
-  Lemma bytes_per_int_gt_0 it : bytes_per_int it > 0.
-  Proof.
-    rewrite /bytes_per_int. move: it => [log ?] /=.
-    rewrite Z2Nat_inj_pow. assert (0 < 2%nat ^ log); last lia.
-    apply Z.pow_pos_nonneg; lia.
-  Qed.
-
-  Definition bits_per_int (it : int_type) : Z :=
-    bytes_per_int it * bits_per_byte.
-
-  Lemma bits_per_int_gt_0 it : bits_per_int it > 0.
-  Proof.
-    rewrite /bits_per_int /bits_per_byte.
-    suff : (bytes_per_int it > 0) by lia.
-    by apply: bytes_per_int_gt_0.
-  Qed.
-
-  Definition int_modulus (it : int_type) : Z :=
-    2 ^ bits_per_int it.
-
-  Definition int_half_modulus (it : int_type) : Z :=
-    2 ^ (bits_per_int it - 1).
-
-  Lemma int_modulus_twice_half_modulus (it : int_type) :
-    int_modulus it = 2 * int_half_modulus it.
-  Proof.
-    rewrite /int_modulus /int_half_modulus.
-    rewrite -[X in X * _]Z.pow_1_r -Z.pow_add_r; try f_equal; try lia.
-    rewrite /bits_per_int /bytes_per_int.
-    apply Z.le_add_le_sub_l. rewrite Z.add_0_r.
-    rewrite Z2Nat_inj_pow.
-    assert (0 < 2%nat ^ it_byte_size_log it * bits_per_byte); last lia.
-    apply Z.mul_pos_pos; last (rewrite /bits_per_byte; lia).
-    apply Z.pow_pos_nonneg; lia.
-  Qed.
-
-  (* Minimal representable integer. *)
-  Definition min_int (it : int_type) : Z :=
-    if it.(it_signed) then - int_half_modulus it else 0.
-
-  (* Maximal representable integer. *)
-  Definition max_int (it : int_type) : Z :=
-    (if it.(it_signed) then int_half_modulus it else int_modulus it) - 1.
-
-  Lemma min_int_le_0 (it : int_type) : min_int it ≤ 0.
-  Proof.
-    have ? := bytes_per_int_gt_0 it. rewrite /min_int /int_half_modulus.
-    destruct (it_signed it) => //. trans (- 2 ^ 7) => //.
-    rewrite -Z.opp_le_mono. apply Z.pow_le_mono_r => //.
-    rewrite /bits_per_int /bits_per_byte. lia.
-  Qed.
-
-  Lemma max_int_ge_127 (it : int_type) : 127 ≤ max_int it.
-  Proof.
-    have ? := bytes_per_int_gt_0 it.
-    rewrite /max_int /int_modulus /int_half_modulus.
-    rewrite /bits_per_int /bits_per_byte.
-    have ->: (127 = 2 ^ 7 - 1) by []. apply Z.sub_le_mono => //.
-    destruct (it_signed it); apply Z.pow_le_mono_r; lia.
-  Qed.
-
-  Global Instance int_elem_of_it : ElemOf Z int_type :=
-    λ z it, min_int it ≤ z ≤ max_int it.
-
-  Lemma int_modulus_mod_in_range n it:
-    it_signed it = false →
-    (n `mod` int_modulus it) ∈ it.
-  Proof.
-    move => ?.
-    have [|??]:= Z.mod_pos_bound n (int_modulus it). {
-      apply: Z.pow_pos_nonneg => //. rewrite /bits_per_int/bits_per_byte/=. lia.
-    }
-    destruct it as [? []] => //.
-    split; unfold min_int, max_int => /=; lia.
-  Qed.
-
-  Definition it_layout (it : int_type) :=
-    Layout (bytes_per_int it) it.(it_byte_size_log).
-
-  Definition i8  := IntType 0 true.
-  Definition u8  := IntType 0 false.
-  Definition i16 := IntType 1 true.
-  Definition u16 := IntType 1 false.
-  Definition i32 := IntType 2 true.
-  Definition u32 := IntType 2 false.
-  Definition i64 := IntType 3 true.
-  Definition u64 := IntType 3 false.
-
-  (* hardcoding 64bit pointers for now *)
-  Definition bytes_per_addr_log : nat := 3%nat.
-  Definition bytes_per_addr : nat := (2 ^ bytes_per_addr_log)%nat.
-
-  Definition intptr_t  := IntType bytes_per_addr_log true.
-  Definition uintptr_t := IntType bytes_per_addr_log false.
-
-  Definition size_t  := uintptr_t.
-  Definition ssize_t := intptr_t.
-  Definition bool_it := u8.
-End IntType.
+(** * Locations *)
 
 Declare Scope loc_scope.
 Delimit Scope loc_scope with L.
 Open Scope loc_scope.
 
-Definition alloc_id := Z.
+(** Physical address. *)
 Definition addr := Z.
 
+(** Allocation identifier (unique to an allocation). *)
+Definition alloc_id := Z.
 Definition dummy_alloc_id : alloc_id := 0.
 
+(** Memory location. *)
 Definition loc : Set := option alloc_id * addr.
 Bind Scope loc_scope with loc.
 
+Definition shift_loc (l : loc) (z : Z) : loc := (l.1, l.2 + z).
+Notation "l +ₗ z" := (shift_loc l%L z%Z)
+  (at level 50, left associativity) : loc_scope.
+Typeclasses Opaque shift_loc.
+
+Definition offset_loc (l : loc) (ly : layout) (z : Z) : loc := (l +ₗ ly.(ly_size) * z).
+Notation "l 'offset{' ly '}ₗ' z" := (offset_loc l%L ly z%Z)
+  (at level 50, format "l  'offset{' ly '}ₗ'  z", left associativity) : loc_scope.
+Typeclasses Opaque offset_loc.
+
+Definition aligned_to (l : loc) (n : nat) : Prop := (n | l.2).
+Notation "l `aligned_to` n" := (aligned_to l n) (at level 50) : stdpp_scope.
+Arguments aligned_to : simpl never.
+Typeclasses Opaque aligned_to.
+
+Definition has_layout_loc (l : loc) (ly : layout) : Prop := l `aligned_to` ly_align ly.
+Notation "l `has_layout_loc` n" := (has_layout_loc l n) (at level 50) : stdpp_scope.
+Arguments has_layout_loc : simpl never.
+Typeclasses Opaque has_layout_loc.
+
+Section loc_lemmas.
+  (*+ Lemmas about [shift_loc] and [offset_loc] *)
+  Lemma shift_loc_assoc l n1 n2 : l +ₗ n1 +ₗ n2 = l +ₗ (n1 + n2).
+  Proof. rewrite /shift_loc /=. f_equal. lia. Qed.
+
+  Lemma shift_loc_0 l : l +ₗ 0 = l.
+  Proof. destruct l as [??]. by rewrite /shift_loc Z.add_0_r. Qed.
+
+  Lemma shift_loc_assoc_nat l (n1 n2 : nat) : l +ₗ n1 +ₗ n2 = l +ₗ (n1 + n2)%nat.
+  Proof. rewrite /shift_loc /=. f_equal. lia. Qed.
+
+  Lemma shift_loc_0_nat l : l +ₗ 0%nat = l.
+  Proof. have: Z.of_nat 0%nat = 0 by lia. move => ->. apply shift_loc_0. Qed.
+
+  Lemma shift_loc_S l n: l +ₗ S n = (l +ₗ 1%nat +ₗ n).
+  Proof. by rewrite shift_loc_assoc_nat. Qed.
+
+  Lemma shift_loc_inj1 l1 l2 n : l1 +ₗ n = l2 +ₗ n → l1 = l2.
+  Proof. destruct l1, l2. case => -> ?. f_equal. lia. Qed.
+
+  Global Instance shift_loc_inj2 l : Inj (=) (=) (shift_loc l).
+  Proof. destruct l as [b o]; intros n n' [=?]; lia. Qed.
+
+  Lemma shift_loc_block l n : (l +ₗ n).1 = l.1.
+  Proof. done. Qed.
+
+  Lemma offset_loc_0 l ly : l offset{ly}ₗ 0 = l.
+  Proof. by rewrite /offset_loc Z.mul_0_r shift_loc_0. Qed.
+
+  Lemma offset_loc_S l ly n : l offset{ly}ₗ S n = (l offset{ly}ₗ 1) offset{ly}ₗ n.
+  Proof. destruct l. rewrite /offset_loc /shift_loc /=. f_equal. lia. Qed.
+
+  Lemma offset_loc_1 l ly : l offset{ly}ₗ 1%nat = (l +ₗ ly.(ly_size)).
+  Proof. destruct l. rewrite /offset_loc /shift_loc /=. f_equal. lia. Qed.
+
+  Lemma offset_loc_sz1 ly l n : ly.(ly_size) = 1%nat → l offset{ly}ₗ n = l +ₗ n.
+  Proof. rewrite /offset_loc => ->. f_equal. lia. Qed.
+
+  (*+ Lemmas about [aligned_to] and [has_layout_loc] *)
+  Lemma ly_with_align_aligned_to l m n:
+    l `aligned_to` n →
+    is_power_of_two n →
+    l `has_layout_loc` ly_with_align m n.
+  Proof. move => ??. by rewrite /has_layout_loc ly_align_ly_with_align keep_factor2_is_power_of_two. Qed.
+
+  Lemma has_layout_loc_trans l ly1 ly2 :
+    l `has_layout_loc` ly2 → (ly1.(ly_align_log) ≤ ly2.(ly_align_log))%nat → l `has_layout_loc` ly1.
+  Proof. rewrite /has_layout_loc/aligned_to => Hl ?. etrans;[|by apply Hl]. by apply Zdivide_nat_pow. Qed.
+
+  Lemma has_layout_loc_trans' l ly1 ly2 :
+    l `has_layout_loc` ly2 → (ly_align ly1 ≤ ly_align ly2)%nat → l `has_layout_loc` ly1.
+  Proof. rewrite -ly_align_log_ly_align_le_iff. by apply: has_layout_loc_trans. Qed.
+
+  Lemma has_layout_loc_1 l ly:
+    ly_align ly = 1%nat →
+    l `has_layout_loc` ly.
+  Proof. rewrite /has_layout_loc =>  ->. by apply Z.divide_1_l. Qed.
+
+  Lemma has_layout_ly_offset l (n : nat) ly:
+    l `has_layout_loc` ly →
+    (l +ₗ n) `has_layout_loc` ly_offset ly n.
+  Proof.
+    move => Hl. apply Z.divide_add_r.
+    - apply: has_layout_loc_trans => //. rewrite {1}/ly_align_log/=. destruct n; lia.
+    - rewrite/ly_offset. destruct n;[by subst;apply Z.divide_0_r|]. etrans;[apply Zdivide_nat_pow, Min.le_min_r|].   by apply factor2_divide.
+  Qed.
+
+  Lemma has_layout_loc_ly_mult_offset l ly n:
+    layout_wf ly →
+    l `has_layout_loc` ly_mult ly (S n) →
+    (l +ₗ ly_size ly) `has_layout_loc` ly_mult ly n.
+  Proof. move => ??. rewrite /ly_mult. by apply Z.divide_add_r. Qed.
+
+
+  Lemma aligned_to_offset l n off :
+    l `aligned_to` n → (n | off) → (l +ₗ off) `aligned_to` n.
+  Proof. apply Z.divide_add_r. Qed.
+
+  Lemma aligned_to_add l (n : nat) x:
+    (l +ₗ x * n) `aligned_to` n ↔ l `aligned_to` n.
+  Proof.
+    unfold aligned_to. destruct l => /=. rewrite Z.add_comm.
+    split.
+    - apply: Z.divide_add_cancel_r. by apply Z.divide_mul_r.
+    - apply Z.divide_add_r. by apply Z.divide_mul_r.
+  Qed.
+
+  Lemma aligned_to_mult_eq l n1 n2 off:
+    l `aligned_to` n2 → (l +ₗ off) `aligned_to` (n1 * n2) → (n2 | off).
+  Proof.
+    unfold aligned_to. destruct l => /= ??. apply: Z.divide_add_cancel_r => //.
+    apply: (Zdivide_mult_l _ n1). by rewrite Z.mul_comm -Nat2Z.inj_mul.
+  Qed.
+End loc_lemmas.
+
+(** * Bytes and values stored in memory *)
+
+(** Representation of a byte stored in memory. *)
 Inductive mbyte : Set :=
 | MByte (b : byte)
 | MPtrFrag (l : loc) (n : nat)
 | MPoison.
 
+(** Representation of a value (list of bytes). *)
 Definition val : Set := list mbyte.
 Bind Scope val_scope with val.
 
+Definition has_layout_val (v : val) (ly : layout) : Prop := length v = ly.(ly_size).
+Notation "v `has_layout_val` n" := (has_layout_val v n) (at level 50) : stdpp_scope.
+Arguments has_layout_val : simpl never.
+Typeclasses Opaque has_layout_val.
+
+(** * Representation of the heap *)
+
 Inductive lock_state := WSt | RSt (n : nat).
 
-Definition heap := gmap addr (alloc_id * lock_state * mbyte).
+Record heap_cell := HeapCell {
+  hc_alloc_id   : alloc_id;   (** Allocation owning the cell. *)
+  hc_lock_state : lock_state; (** Datarace detection stuff. *)
+  hc_value      : mbyte;      (** Byte value. *)
+}.
+
+Definition heap := gmap addr heap_cell.
+
+(** Predicate stating that the heap [h] contains value [v] at address [a],
+and that every cell involved has an allocation identifier and a lock state
+that satisfy [Paid] and [Plk] respectively. *)
+Fixpoint heap_lookup (a : addr) (v : val) (Paid : alloc_id → Prop)
+                       (Plk : lock_state → Prop) (h : heap) : Prop :=
+  match v with
+  | []     => True
+  | b :: v => (∃ aid lk, h !! a = Some (HeapCell aid lk b) ∧ Paid aid ∧ Plk lk) ∧
+              heap_lookup (Z.succ a) v Paid Plk h
+  end.
+
+(** Function writing value [v] at address [a] in heap [h]. For all involved
+cells in the resulting heap, an allocation id and lock state is built using
+functions [faid] and [flk] respectively. These functions receive as input
+the previous value of the field (if the cell previously existed in [h]). *)
+Fixpoint heap_update (a : addr) (v : val) (faid : option alloc_id → alloc_id)
+                     (flk : option lock_state → lock_state) (h : heap) : heap :=
+  match v with
+  | []     => h
+  | b :: v => let update m :=
+                Some {|
+                  hc_alloc_id   := faid (hc_alloc_id <$> m);
+                  hc_lock_state := flk (hc_lock_state <$> m);
+                  hc_value      := b;
+                |}
+              in
+              partial_alter update a (heap_update (Z.succ a) v faid flk h)
+  end.
+
+Definition heap_lookup_loc (l : loc) (v : val) (Plk : lock_state → Prop)
+                             (h : heap) : Prop :=
+  heap_lookup l.2 v (λ aid, l.1 = Some aid) Plk h.
+
+Definition heap_alloc (a : addr) (v : val) (aid : alloc_id) (h : heap) : heap :=
+  heap_update a v (λ _, aid) (λ _, RSt 0%nat) h.
+
+(** Predicate stating that the allocation [aid] is still present in heap [h]. *)
+Definition heap_block_alive (h : heap) (aid : alloc_id) : Prop :=
+  ∃ a, hc_alloc_id <$> h !! a = Some aid.
+
+Definition heap_at (l : loc) (ly : layout) (v : val) (Plk : lock_state → Prop)
+                   (h : heap) : Prop :=
+  is_Some l.1 ∧ l `has_layout_loc` ly ∧ v `has_layout_val` ly ∧
+  heap_lookup_loc l v Plk h.
+
+Definition heap_upd l v flk h :=
+  heap_update l.2 v (λ _, default dummy_alloc_id l.1) flk h.
+
+(** Predicate stating that the [n] first bytes from address [a] in [h] have
+not been allocated. *)
+Definition heap_range_free (h : heap) (a : addr) (n : nat) : Prop :=
+  ∀ a', a ≤ a' < a + n → h !! a' = None.
+
+(** Free [n] cells starting at [a] in [h]. *)
+Fixpoint heap_free (a : addr) (n : nat) (h : heap) : heap :=
+  match n with
+  | O   => h
+  | S n => delete a (heap_free (Z.succ a) n h)
+  end.
+
+Fixpoint heap_free_list (ls : list (loc * layout)) (h : heap) : heap :=
+  match ls with
+  | []           => h
+  | (l,ly) :: ls => heap_free l.2 ly.(ly_size) (heap_free_list ls h)
+  end.
+
+Section heap_lemmas.
+  Lemma heap_lookup_inj_val a h v1 v2 Paid1 Paid2 Plk1 Plk2:
+    length v1 = length v2 →
+    heap_lookup a v1 Paid1 Plk1 h → heap_lookup a v2 Paid2 Plk2 h → v1 = v2.
+  Proof.
+    elim: v1 v2 a; first by move => [|??] //.
+    move => ?? IH [|??] //= ? [?] [[?[?[??]]]?] [[?[?[??]]]?]; simplify_eq.
+    f_equal. by apply: IH.
+  Qed.
+
+  Lemma heap_update_ext h a v faid1 faid2 flk1 flk2:
+    (∀ x, faid1 x = faid2 x) → (∀ x, flk1 x = flk2 x) →
+    heap_update a v faid1 flk1 h = heap_update a v faid2 flk2 h.
+  Proof.
+    move => Hext1 Hext2. elim: v a => //= ?? IH ?. rewrite IH.
+    apply: partial_alter_ext => ??. by rewrite Hext1 Hext2.
+  Qed.
+
+  Lemma heap_update_lookup_lt a1 a2 v faid flk h:
+    a1 < a2 →
+    heap_update a2 v faid flk h !! a1 = h !! a1.
+  Proof.
+    elim: v a1 a2 => // ?? IH ???.
+    rewrite lookup_partial_alter_ne; last lia. apply IH. lia.
+  Qed.
+
+  Lemma heap_free_delete h a1 a2 n :
+    delete a1 (heap_free a2 n h) = heap_free a2 n (delete a1 h).
+  Proof. elim: n a2 => //= ? IH ?. by rewrite delete_commute IH. Qed.
+
+  Lemma heap_free_list_app ls1 ls2 h :
+    heap_free_list (ls1 ++ ls2) h = heap_free_list ls1 (heap_free_list ls2 h).
+  Proof. by elim: ls1 => //= [[??]] ? ->. Qed.
+
+  Lemma heap_upd_ext h l v f1 f2:
+    (∀ x, f1 x = f2 x) → heap_upd l v f1 h = heap_upd l v f2 h.
+  Proof. by apply heap_update_ext. Qed.
+
+  Lemma heap_at_inj_val l ly h v1 v2 Plk1 Plk2:
+    heap_at l ly v1 Plk1 h → heap_at l ly v2 Plk2 h → v1 = v2.
+  Proof.
+    move => [_[?[??]]] [_[?[??]]].
+    apply: heap_lookup_inj_val => //. congruence.
+  Qed.
+
+  Lemma heap_lookup_loc_inj_val  l h v v' flk1 flk2 ly:
+    v `has_layout_val` ly →
+    heap_lookup_loc l v flk1 h → heap_at l ly v' flk2 h → v = v'.
+  Proof.
+    move => ??[_[?[??]]]. apply: heap_lookup_inj_val => //. congruence.
+  Qed.
+
+  Lemma heap_upd_heap_at_id l v flk flk' h:
+    heap_lookup_loc l v flk' h →
+    (∀ st, flk (Some st) = st) →
+    heap_upd l v flk h = h.
+  Proof.
+    rewrite /heap_upd.
+    elim: v l => // ?? IH ? [[?[?[H[H1 ?]]]]?] Hlookup /=.
+    assert (∀ l, Z.succ l.2 = (l +ₗ 1).2) as -> by done.
+    rewrite IH => //. apply: partial_alter_self_alt'.
+    by rewrite H Hlookup H1 /=.
+  Qed.
+End heap_lemmas.
+
+(** * Allocations and heap state *)
 
 Record allocation :=
   Allocation {
@@ -260,33 +308,64 @@ Record allocation :=
 
 Definition allocs := gmap alloc_id allocation.
 
+Record heap_state := {
+  hs_heap   : heap;
+  hs_allocs : allocs;
+}.
 
+(** Smallest allocatble address (we reserve 0 for NULL). *)
+Definition min_alloc_start : Z := 1.
 
-Definition shift_loc (l : loc) (z : Z) : loc := (l.1, l.2 + z).
-Notation "l +ₗ z" := (shift_loc l%L z%Z)
-  (at level 50, left associativity) : loc_scope.
-Definition offset_loc (l : loc) (ly : layout) (z : Z) : loc := (l +ₗ ly.(ly_size) * z).
-Notation "l 'offset{' ly '}ₗ' z" := (offset_loc l%L ly z%Z)
-  (at level 50, format "l  'offset{' ly '}ₗ'  z", left associativity) : loc_scope.
+(** Largest allocatable address (we never allocate the last byte to always
+have valid one-past pointers. *)
+Definition max_alloc_end : Z := 2 ^ (bytes_per_addr * bits_per_byte) - 2.
 
-Typeclasses Opaque shift_loc offset_loc.
+Definition to_allocation (off : Z) (len : nat) : allocation :=
+  Allocation off (off + len).
 
-Definition aligned_to (l : loc) (n : nat) : Prop := (n | l.2).
-Notation "l `aligned_to` n" := (aligned_to l n) (at level 50) : stdpp_scope.
-Definition has_layout_loc (l : loc) (ly : layout) : Prop := l `aligned_to` ly_align ly.
-Notation "l `has_layout_loc` n" := (has_layout_loc l n) (at level 50) : stdpp_scope.
-Definition has_layout_val (v : val) (ly : layout) : Prop := length v = ly.(ly_size).
-Notation "v `has_layout_val` n" := (has_layout_val v n) (at level 50) : stdpp_scope.
+Definition allocation_in_range (a : allocation) : Prop :=
+  min_alloc_start ≤ a.(alloc_start) ∧ a.(alloc_end) ≤ max_alloc_end.
 
-Arguments aligned_to : simpl never.
-(* Arguments aligned_to_log : simpl never. *)
-Arguments has_layout_loc : simpl never.
-Arguments has_layout_val : simpl never.
-Typeclasses Opaque aligned_to has_layout_loc has_layout_val.
+(** The address range between [l] and [l +ₗ n] (included) is in range of the
+    allocation that contains [l]. Note that we consider the 1-past-the-end
+    pointer to be in range of an allocation. *)
+Definition heap_state_loc_in_bounds (l : loc) (n : nat) (st : heap_state) : Prop :=
+  ∃ alloc_id alloc,
+    l.1 = Some alloc_id ∧
+    st.(hs_allocs) !! alloc_id = Some alloc ∧
+    alloc.(alloc_start) ≤ l.2 ∧
+    l.2 + n ≤ alloc.(alloc_end).
 
+(** Checks that the location [l] is inbounds of its allocation
+(one-past-the-end is allowed) and this allocation is still alive *)
+Definition valid_ptr (l : loc) (st : heap_state) : Prop :=
+  ∃ aid, l.1 = Some aid ∧ heap_block_alive st.(hs_heap) aid ∧ heap_state_loc_in_bounds l 0 st.
 
-(*** Definitions of the language *)
-Definition label := string. (* make TC opaque and implement countable and eqdicision *)
+Inductive alloc_new_block : heap_state → loc → val → heap_state → Prop :=
+| AllocNewBlock σ l aid v:
+    l.1 = Some aid →
+    σ.(hs_allocs) !! aid = None →
+    (* TODO: is the precondition really useful? It should follow from
+    the previous. *)
+    ¬ heap_block_alive σ.(hs_heap) aid →
+    allocation_in_range (to_allocation l.2 (length v)) →
+    heap_range_free σ.(hs_heap) l.2 (length v) →
+    alloc_new_block σ l v {|
+      hs_heap   := heap_alloc l.2 v aid σ.(hs_heap);
+      hs_allocs := <[aid := to_allocation l.2 (length v)]> σ.(hs_allocs);
+    |}.
+
+Inductive alloc_new_blocks : heap_state → list loc → list val → heap_state → Prop :=
+| AllocNewBlock_nil σ :
+    alloc_new_blocks σ [] [] σ
+| AllocNewBlock_cons σ σ' σ'' l v ls vs :
+    alloc_new_block σ l v σ' →
+    alloc_new_blocks σ' ls vs σ'' →
+    alloc_new_blocks σ (l :: ls) (v :: vs) σ''.
+
+(** * Definition of the language *)
+
+Definition label := string.
 Definition var_name := string.
 
 Inductive op_type : Set :=
@@ -371,12 +450,16 @@ Record function := {
   f_init : label;
 }.
 
-(* TODO: put both function and bytes in the same heap or make pointers disjoint (current version is wrong)*)
+(* TODO: put both function and bytes in the same heap or make pointers disjoint *)
 Record state := {
-  st_heap: heap;
-  st_allocs: allocs;
+  st_heap: heap_state;
   st_fntbl: gmap loc function;
 }.
+
+Definition heap_fmap (f : heap → heap) (σ : state) := {|
+  st_heap := {| hs_heap := f σ.(st_heap).(hs_heap); hs_allocs := σ.(st_heap).(hs_allocs) |};
+  st_fntbl := σ.(st_fntbl);
+|}.
 
 Record runtime_function := {
   (* locations of args and local vars are substitued in the body *)
@@ -459,6 +542,7 @@ Proof. move => ? s1 ? s2 [-> ]. elim: s1 s2 => [ ^ e1 ] [ ^ e2 ] // ?; simplify_
 Implicit Type (l : loc) (re : rtexpr) (v : val) (sz : nat) (h : heap) (σ : state) (ly : layout) (rs : rtstmt) (s : stmt) (sgn : signed) (rf : runtime_function).
 
 (*** Relating val to logical values *)
+(*+ [val_to_int] and [val_of_int] *)
 (* we use little endian *)
 Fixpoint val_to_int_go v : option Z :=
 match v with
@@ -543,15 +627,7 @@ Proof.
     + rewrite /int_modulus /bits_per_int in HM. lia.
 Qed.
 
-Lemma it_in_range_mod n it:
-  n ∈ it → it_signed it = false →
-  n `mod` int_modulus it = n.
-Proof.
-  move => [??] ?. rewrite Z.mod_small //.
-  destruct it as [? []] => //. unfold min_int, max_int in *. simpl in *.
-  lia.
-Qed.
-
+(*+ [val_to_loc] and [val_of_loc] *)
 Fixpoint val_to_loc_go (v : val) (pos : nat) (l : loc) : option loc :=
   match v with
   | (MPtrFrag l' pos')::v' =>
@@ -582,6 +658,7 @@ Proof.
   by case_match => // [[->]].
 Qed.
 
+(*+ [val_of_bool] and [i2v] *)
 Definition i2v (n : Z) (it : int_type) : val := default [MPoison] (val_of_int n it).
 
 Definition val_of_bool (b : bool) : val := i2v (Z_of_bool b) bool_it.
@@ -595,6 +672,10 @@ Proof.
   split; destruct b => /=; lia.
 Qed.
 
+Lemma val_to_int_bool b :
+  val_to_int (val_of_bool b) bool_it = Some (Z_of_bool b).
+Proof. by destruct b. Qed.
+
 Lemma i2v_bool_length b it:
   length (i2v (Z_of_bool b) it) = bytes_per_int it.
 Proof. by have /val_of_int_length -> := val_of_int_bool b it. Qed.
@@ -607,198 +688,6 @@ Arguments val_of_int : simpl never.
 Arguments val_to_loc : simpl never.
 Arguments val_of_loc : simpl never.
 Typeclasses Opaque val_to_loc val_of_loc val_to_int val_of_int val_of_bool.
-
-
-Lemma val_to_int_bool b :
-  val_to_int (val_of_bool b) bool_it = Some (Z_of_bool b).
-Proof. by destruct b. Qed.
-
-Definition zero_val (n : nat) : val :=
-  replicate n (MByte byte0).
-Arguments zero_val : simpl never.
-Typeclasses Opaque zero_val.
-
-(*** Properties of layouts and alignment *)
-Lemma ly_align_log_ly_align_eq_iff ly1 ly2:
-  ly_align_log ly1 = ly_align_log ly2 ↔ ly_align ly1 = ly_align ly2.
-Proof. rewrite /ly_align. split; first naive_solver. move => /Nat.pow_inj_r. lia. Qed.
-
-Lemma ly_align_log_ly_align_le_iff ly1 ly2:
-  (ly_align_log ly1 ≤ ly_align_log ly2 ↔ ly_align ly1 ≤ ly_align ly2)%nat.
-Proof. rewrite /ly_align. apply: Nat.pow_le_mono_r_iff. lia. Qed.
-
-Lemma ly_size_ly_with_align m n :
-  ly_size (ly_with_align m n) = m.
-Proof. done. Qed.
-
-Lemma ly_align_ly_with_align m n :
-  ly_align (ly_with_align m n) = keep_factor2 n 1.
-Proof. rewrite /ly_with_align/keep_factor2/factor2. by destruct (factor2' n). Qed.
-
-Lemma ly_align_ly_offset ly n :
-  ly_align (ly_offset ly n) = (ly_align ly `min` keep_factor2 n (ly_align ly))%nat.
-Proof.
-  rewrite /ly_align/keep_factor2/=/factor2. destruct (factor2' n) as [n'|] => /=; last by rewrite !Nat.min_id.
-  destruct (decide (ly_align_log ly ≤ n'))%nat;[rewrite !min_l|rewrite !min_r]; try lia;
-    apply Nat.pow_le_mono_r; lia.
-Qed.
-
-Lemma ly_size_ly_set_size ly n:
-  ly_size (ly_set_size ly n) = n.
-Proof. done. Qed.
-
-Lemma ly_align_ly_set_size ly n:
-  ly_align (ly_set_size ly n) = ly_align ly.
-Proof. done. Qed.
-
-Lemma ly_with_align_aligned_to l m n:
-  l `aligned_to` n →
-  is_power_of_two n →
-  l `has_layout_loc` ly_with_align m n.
-Proof. move => ??. by rewrite /has_layout_loc ly_align_ly_with_align keep_factor2_is_power_of_two. Qed.
-
-Lemma has_layout_loc_trans l ly1 ly2 :
-  l `has_layout_loc` ly2 → (ly1.(ly_align_log) ≤ ly2.(ly_align_log))%nat → l `has_layout_loc` ly1.
-Proof. rewrite /has_layout_loc/aligned_to => Hl ?. etrans;[|by apply Hl]. by apply Zdivide_nat_pow. Qed.
-
-Lemma has_layout_loc_trans' l ly1 ly2 :
-  l `has_layout_loc` ly2 → (ly_align ly1 ≤ ly_align ly2)%nat → l `has_layout_loc` ly1.
-Proof. rewrite -ly_align_log_ly_align_le_iff. by apply: has_layout_loc_trans. Qed.
-
-Lemma has_layout_loc_1 l ly:
-  ly_align ly = 1%nat →
-  l `has_layout_loc` ly.
-Proof. rewrite /has_layout_loc =>  ->. by apply Z.divide_1_l. Qed.
-
-Lemma has_layout_ly_offset l (n : nat) ly:
-  l `has_layout_loc` ly →
-  (l +ₗ n) `has_layout_loc` ly_offset ly n.
-Proof.
-  move => Hl. apply Z.divide_add_r.
-  - apply: has_layout_loc_trans => //. rewrite {1}/ly_align_log/=. destruct n; lia.
-  - rewrite/ly_offset. destruct n;[by subst;apply Z.divide_0_r|]. etrans;[apply Zdivide_nat_pow, Min.le_min_r|]. by apply factor2_divide.
-Qed.
-
-Lemma has_layout_loc_ly_mult_offset l ly n:
-  layout_wf ly →
-  l `has_layout_loc` ly_mult ly (S n) →
-  (l +ₗ ly_size ly) `has_layout_loc` ly_mult ly n.
-Proof. move => ??. rewrite /ly_mult. by apply Z.divide_add_r. Qed.
-
-
-Lemma aligned_to_offset l n off :
-  l `aligned_to` n → (n | off) → (l +ₗ off) `aligned_to` n.
-Proof. apply Z.divide_add_r. Qed.
-
-Lemma aligned_to_add l (n : nat) x:
-  (l +ₗ x * n) `aligned_to` n ↔ l `aligned_to` n.
-Proof.
-  unfold aligned_to. destruct l => /=. rewrite Z.add_comm.
-  split.
-  - apply: Z.divide_add_cancel_r. by apply Z.divide_mul_r.
-  - apply Z.divide_add_r. by apply Z.divide_mul_r.
-Qed.
-
-Lemma aligned_to_mult_eq l n1 n2 off:
-  l `aligned_to` n2 → (l +ₗ off) `aligned_to` (n1 * n2) → (n2 | off).
-Proof.
-  unfold aligned_to. destruct l => /= ??. apply: Z.divide_add_cancel_r => //.
-  apply: (Zdivide_mult_l _ n1). by rewrite Z.mul_comm -Nat2Z.inj_mul.
-Qed.
-
-(*** Helper functions for accessing the heap *)
-
-(* The address range between [l] and [l +ₗ n] (included) is in range of the
-   allocation that contains [l]. Note that we consider the 1-past-the-end
-   pointer to be in range of an allocation. *)
-Definition heap_loc_in_bounds (l : loc) (n : nat) (st : state) : Prop :=
-  ∃ alloc_id alloc,
-    l.1 = Some alloc_id ∧
-    st.(st_allocs) !! alloc_id = Some alloc ∧
-    alloc.(alloc_start) ≤ l.2 ∧
-    l.2 + n ≤ alloc.(alloc_end).
-
-Fixpoint heap_at_go l v flk h : Prop :=
-  match v with
-  | [] => True
-  | b::v' => (∃ lk, h !! l.2 = Some (default dummy_alloc_id l.1, lk, b) ∧ flk lk) ∧ heap_at_go (l +ₗ 1) v' flk h
-  end.
-
-Definition heap_at l ly v flk h : Prop :=
-  is_Some l.1 ∧ l `has_layout_loc` ly ∧ v `has_layout_val` ly ∧ heap_at_go l v flk h.
-
-Definition heap_block_alive (h : heap) (aid : alloc_id) : Prop :=
-  ∃ a lk b, h !! a = Some (aid, lk, b).
-
-Definition heap_range_free (h : heap) (a : addr) (n : nat) : Prop :=
-  ∀ a', a ≤ a' < a + n → h !! a' = None.
-
-Fixpoint heap_upd l v (flk : option lock_state → lock_state) (h : heap) : heap :=
-  match v with
-  | b::v' => partial_alter (λ m, Some (default dummy_alloc_id l.1,
-                                       flk (snd <$> (fst <$> m)), b)) l.2 (heap_upd (l +ₗ 1) v' flk h)
-  | [] => h
-  end.
-
-Fixpoint heap_upd_list ls vs flk h : heap :=
-  match ls, vs with
-  | l::ls', v::vs' => heap_upd l v flk (heap_upd_list ls' vs' flk h)
-  | _, _ => h
-  end.
-
-Fixpoint heap_free l n h : heap :=
-  match n with
-  | O => h
-  | S n' => delete l.2 (heap_free (l +ₗ 1) n' h)
-  end.
-
-Fixpoint heap_free_list ls h : heap :=
-  match ls with
-  | (l, ly)::ls' => heap_free l ly.(ly_size) (heap_free_list ls' h)
-  | _ => h
-  end.
-
-Definition heap_fmap f σ := {|
-  st_heap := f σ.(st_heap);
-  st_fntbl := σ.(st_fntbl);
-  st_allocs := σ.(st_allocs);
-|}.
-
-(*** Allocation semantics *)
-(* We reserve 0 for NULL. *)
-Definition min_alloc_start : Z := 1.
-
-(* We never allocate the last byte to always have valid one-past pointers. *)
-Definition max_alloc_end   : Z := 2 ^ (bytes_per_addr * bits_per_byte) - 2.
-
-Definition to_allocation (off : Z) (len : nat) : allocation :=
-  Allocation off (off + len).
-
-Definition allocation_in_range (a : allocation) : Prop :=
-  min_alloc_start ≤ a.(alloc_start) ∧ a.(alloc_end) ≤ max_alloc_end.
-
-Inductive alloc_new_block : state → loc → val → state → Prop :=
-| AllocNewBlock σ l aid v:
-    l.1 = Some aid →
-    σ.(st_allocs) !! aid = None →
-    (* TODO: is the precondition really useful? It should follow from
-    the previous. *)
-    ¬ heap_block_alive σ.(st_heap) aid →
-    allocation_in_range (to_allocation l.2 (length v)) →
-    heap_range_free σ.(st_heap) l.2 (length v) →
-    alloc_new_block σ l v {|
-      st_heap   := heap_upd l v (λ _, RSt 0%nat) σ.(st_heap);
-      st_allocs := <[aid := to_allocation l.2 (length v)]> σ.(st_allocs);
-      st_fntbl  := σ.(st_fntbl);
-    |}.
-
-Inductive alloc_new_blocks : state → list loc → list val → state → Prop :=
-| AllocNewBlock_nil σ :
-    alloc_new_blocks σ [] [] σ
-| AllocNewBlock_cons σ σ' σ'' l v ls vs :
-    alloc_new_block σ l v σ' →
-    alloc_new_blocks σ' ls vs σ'' →
-    alloc_new_blocks σ (l :: ls) (v :: vs) σ''.
 
 (*** Substitution *)
 Fixpoint subst (x : var_name) (v : val) (e : expr)  : expr :=
@@ -840,10 +729,6 @@ Definition subst_function (xs : list (var_name * val)) (f : function) : function
 |}.
 
 (*** Evaluation of operations *)
-(** Checks that the location [l] is inbounds of its allocation
-(one-past-the-end is allowed) and this allocation is still alive *)
-Definition valid_ptr (l : loc) (st : state) : Prop :=
-  ∃ aid, l.1 = Some aid ∧ heap_block_alive st.(st_heap) aid ∧ heap_loc_in_bounds l 0 st.
 
 (* evaluation can be non-deterministic for comparing pointers *)
 Inductive eval_bin_op : bin_op → op_type → op_type → state → val → val → val → Prop :=
@@ -859,14 +744,14 @@ Inductive eval_bin_op : bin_op → op_type → op_type → state → val → val
     (* TODO: should we have an alignment check here? *)
     eval_bin_op (PtrNegOffsetOp ly) (IntOp it) PtrOp σ v1 v2 (val_of_loc (l offset{ly}ₗ -o))
 | EqOpPNull v1 v2 σ l v:
-    heap_loc_in_bounds l 0%nat σ →
+    heap_state_loc_in_bounds l 0%nat σ.(st_heap) →
     val_to_loc v1 = Some l →
     val_to_int v2 size_t = Some 0 →
     (* TODO ( see below ): Should we really hard code i32 here because of C? *)
     i2v (Z_of_bool false) i32 = v →
     eval_bin_op EqOp PtrOp PtrOp σ v1 v2 v
 | NeOpPNull v1 v2 σ l v:
-    heap_loc_in_bounds l 0%nat σ →
+    heap_state_loc_in_bounds l 0%nat σ.(st_heap) →
     val_to_loc v1 = Some l →
     val_to_int v2 size_t = Some 0 →
     i2v (Z_of_bool true) i32 = v →
@@ -884,7 +769,7 @@ Inductive eval_bin_op : bin_op → op_type → op_type → state → val → val
 | RelOpPP v1 v2 σ l1 l2 v b op:
     val_to_loc v1 = Some l1 →
     val_to_loc v2 = Some l2 →
-    valid_ptr l1 σ → valid_ptr l2 σ →
+    valid_ptr l1 σ.(st_heap) → valid_ptr l2 σ.(st_heap) →
     match op with
     | EqOp => Some (bool_decide (l1.2 = l2.2))
     | NeOp => Some (bool_decide (l1.2 ≠ l2.2))
@@ -987,16 +872,16 @@ Inductive expr_step : expr → state → list Empty_set → runtime_expr → sta
     in
     let end_expr := if o is Na1Ord then Deref Na2Ord ly (Val v) else Val v' in
     val_to_loc v = Some l →
-    heap_at l ly v' start_st σ.(st_heap) →
+    heap_at l ly v' start_st σ.(st_heap).(hs_heap) →
     expr_step (Deref o ly (Val v)) σ [] end_expr (heap_fmap (heap_upd l v' end_st) σ) []
 (* TODO: look at CAS and see whether it makes sense. Also allow
 comparing pointers? (see lambda rust) *)
 (* corresponds to atomic_compare_exchange_strong, see https://en.cppreference.com/w/c/atomic/atomic_compare_exchange *)
 | CasFailS l1 l2 vo ve σ z1 z2 v1 v2 v3 it:
     val_to_loc v1 = Some l1 →
-    heap_at l1 (it_layout it) vo (λ st, ∃ n, st = RSt n) σ.(st_heap) →
+    heap_at l1 (it_layout it) vo (λ st, ∃ n, st = RSt n) σ.(st_heap).(hs_heap) →
     val_to_loc v2 = Some l2 →
-    heap_at l2 (it_layout it) ve (λ st, st = RSt 0%nat) σ.(st_heap) →
+    heap_at l2 (it_layout it) ve (λ st, st = RSt 0%nat) σ.(st_heap).(hs_heap) →
     val_to_int vo it = Some z1 →
     val_to_int ve it = Some z2 →
     v3 `has_layout_val` it_layout it →
@@ -1006,9 +891,9 @@ comparing pointers? (see lambda rust) *)
               (Val (val_of_bool false)) (heap_fmap (heap_upd l2 vo (λ _, RSt 0%nat)) σ) []
 | CasSucS l1 l2 it vo ve σ z1 z2 v1 v2 v3:
     val_to_loc v1 = Some l1 →
-    heap_at l1 (it_layout it) vo (λ st, st = RSt 0%nat) σ.(st_heap) →
+    heap_at l1 (it_layout it) vo (λ st, st = RSt 0%nat) σ.(st_heap).(hs_heap) →
     val_to_loc v2 = Some l2 →
-    heap_at l2 (it_layout it) ve (λ st, ∃ n, st = RSt n) σ.(st_heap) →
+    heap_at l2 (it_layout it) ve (λ st, ∃ n, st = RSt n) σ.(st_heap).(hs_heap) →
     val_to_int vo it = Some z1 →
     val_to_int ve it = Some z2 →
     v3 `has_layout_val` it_layout it →
@@ -1029,9 +914,11 @@ comparing pointers? (see lambda rust) *)
     Forall2 has_layout_loc lsa fn.(f_args).*2 →
     Forall2 has_layout_loc lsv fn.(f_local_vars).*2 →
     (* initialize the local vars to poison *)
-    alloc_new_blocks σ lsv ((λ p, replicate p.2.(ly_size) MPoison) <$> fn.(f_local_vars)) σ' →
+    alloc_new_blocks σ.(st_heap) lsv ((λ p, replicate p.2.(ly_size) MPoison) <$> fn.(f_local_vars)) σ'.(st_heap) →
+    σ.(st_fntbl) = σ'.(st_fntbl) →
     (* initialize the arguments with the supplied values *)
-    alloc_new_blocks σ' lsa vs σ'' →
+    alloc_new_blocks σ'.(st_heap) lsa vs σ''.(st_heap) →
+    σ'.(st_fntbl) = σ''.(st_fntbl) →
     (* add used blocks allocations  *)
     rf = {| rf_fn := fn'; rf_locs := zip lsa fn.(f_args).*2 ++ zip lsv fn.(f_local_vars).*2; |} →
     expr_step (Call (Val vf) (Val <$> vs)) σ [] (to_rtstmt rf (Goto fn'.(f_init))) σ'' []
@@ -1061,7 +948,7 @@ Inductive stmt_step : stmt → runtime_function → state → list Empty_set →
     let end_stmt := if o is Na1Ord then Assign Na2Ord ly (Val v1) (Val v2) s else s in
     val_to_loc v1 = Some l →
     v2 `has_layout_val` ly →
-    heap_at l ly v' start_st σ.(st_heap) →
+    heap_at l ly v' start_st σ.(st_heap).(hs_heap) →
     stmt_step (Assign o ly (Val v1) (Val v2) s) rf σ [] (to_rtstmt rf end_stmt) (heap_fmap (heap_upd l end_val end_st) σ) []
 | SwitchS rf σ v n m bs s def it :
     val_to_int v it = Some n →
@@ -1225,113 +1112,18 @@ Canonical Structure c_ectxi_lang := EctxiLanguage c_lang_mixin.
 Canonical Structure c_ectx_lang := EctxLanguageOfEctxi c_ectxi_lang.
 Canonical Structure c_lang := LanguageOfEctx c_ectx_lang.
 
-(*** General lemmata *)
-Lemma Z_of_bool_true b :
-  Z_of_bool b ≠ 0 ↔ b = true.
-Proof. destruct b; naive_solver. Qed.
-
-Lemma Z_of_bool_false b :
-  Z_of_bool b = 0 ↔ b = false.
-Proof. destruct b; naive_solver. Qed.
-
-Lemma shift_loc_assoc l n n' : l +ₗ n +ₗ n' = l +ₗ (n + n').
-Proof. rewrite /shift_loc /=. f_equal. lia. Qed.
-Lemma shift_loc_0 l : l +ₗ 0 = l.
-Proof. destruct l as [b o]. rewrite /shift_loc /=. f_equal. lia. Qed.
-
-Lemma shift_loc_assoc_nat l (n n' : nat) : l +ₗ n +ₗ n' = l +ₗ (n + n')%nat.
-Proof. rewrite /shift_loc /=. f_equal. lia. Qed.
-Lemma shift_loc_0_nat l : l +ₗ 0%nat = l.
-Proof. destruct l as [b o]. rewrite /shift_loc /=. f_equal. lia. Qed.
-
-Lemma shift_loc_S l n: l +ₗ S n = (l +ₗ 1%nat +ₗ n).
-Proof. by rewrite shift_loc_assoc_nat. Qed.
-
-Lemma shift_loc_inj1 l1 l2 n : l1 +ₗ n = l2 +ₗ n → l1 = l2.
-Proof. destruct l1, l2. case => -> ?. f_equal. lia. Qed.
-
-Instance shift_loc_inj2 l : Inj (=) (=) (shift_loc l).
-Proof. destruct l as [b o]; intros n n' [=?]; lia. Qed.
-
-Lemma shift_loc_block l n : (l +ₗ n).1 = l.1.
-Proof. done. Qed.
-
-Lemma offset_loc_0 l ly : l offset{ly}ₗ 0 = l.
-Proof. rewrite /offset_loc/=. have -> : ly_size ly * 0 = 0 by lia. apply shift_loc_0. Qed.
-
-Lemma offset_loc_S l ly n : l offset{ly}ₗ S n = (l offset{ly}ₗ 1) offset{ly}ₗ n.
-Proof. rewrite /offset_loc/shift_loc/=. destruct l => /=. f_equal. lia. Qed.
-
-Lemma offset_loc_1 l ly : l offset{ly}ₗ 1%nat = (l +ₗ ly.(ly_size)).
-Proof. rewrite /offset_loc/shift_loc/=. destruct l => /=. f_equal. lia. Qed.
-
-Lemma offset_loc_sz1 ly l n : ly.(ly_size) = 1%nat → l offset{ly}ₗ n = l +ₗ n.
-Proof. rewrite /offset_loc => ->. f_equal. lia. Qed.
-
-Lemma heap_at_go_inj_val l h v v' flk1 flk2:
-  length v = length v' →
-  heap_at_go l v flk1 h → heap_at_go l v' flk2 h → v = v'.
-Proof.
-  elim: v v' l; first by move => [|??] // ? [[]].
-  move => b v IH [|b' v'] //= l [?] [[?[??]]?] [[?[??]]?]; simplify_eq.
-  f_equal. by apply: IH.
-Qed.
-
-Lemma heap_at_go_inj_val'  l h v v' flk1 flk2 ly:
-  v `has_layout_val` ly →
-  heap_at_go l v flk1 h → heap_at l ly v' flk2 h → v = v'.
-Proof.
-  move => ??[_[?[??]]]. apply: heap_at_go_inj_val => //. congruence.
-Qed.
-
-Lemma heap_at_inj_val l ly h v v' flk1 flk2:
-  heap_at l ly v flk1 h → heap_at l ly v' flk2 h → v = v'.
-Proof.
-  move => [_ [Hv1 [H1 ?]]] [_ [Hv2 [H2 ?]]].
-  apply: heap_at_go_inj_val => //. congruence.
-Qed.
-
-Lemma heap_upd_ext h l v f1 f2:
-  (∀ x, f1 x = f2 x) →
-  heap_upd l v f1 h = heap_upd l v f2 h.
-Proof.
-  move => Hext. elim: v l => //= ?? IH ?. rewrite IH.
-  apply: partial_alter_ext => ??. by rewrite Hext.
-Qed.
-
-Lemma heap_upd_lookup_lt l n bl h flk:
-  n > 0 →
-  heap_upd (l +ₗ n) bl flk h !! l.2 = h !! l.2.
-Proof.
-  elim: bl n => // b bl IH /= n Hn. rewrite shift_loc_assoc.
-  rewrite lookup_partial_alter_ne //.
-  - apply IH. lia.
-  - rewrite /shift_loc. destruct l. lia.
-Qed.
-
-Lemma heap_upd_heap_at_id l v flk flk' h:
-  heap_at_go l v flk' h →
-  (∀ st, flk (Some st) = st) →
-  heap_upd l v flk h = h.
-Proof.
-  elim: v l => //= b v IH l [[lk[Hlk ?]]?] Hflk. rewrite IH //.
-  apply: partial_alter_self_alt'. by rewrite Hlk Hflk.
-Qed.
-
-Lemma heap_free_delete h l l' n :
-  delete l.2 (heap_free l' n h) = heap_free l' n (delete l.2 h).
-Proof. revert l'. induction n as [|n IH]=> l' //=. by rewrite delete_commute IH. Qed.
-
-Lemma heap_free_list_app ls1 ls2 h:
-  heap_free_list (ls1 ++ ls2) h = heap_free_list ls1 (heap_free_list ls2 h).
-Proof. by elim: ls1 => //= [[??]] ? ->. Qed.
+(** * Useful instances and canonical structures *)
 
 Instance mbyte_inhabited : Inhabited mbyte := populate (MPoison).
 Instance val_inhabited : Inhabited val := _.
 Instance expr_inhabited : Inhabited expr := populate (Val inhabitant).
 Instance stmt_inhabited : Inhabited stmt := populate (Goto "a").
-Instance function_inhabited : Inhabited function := populate {| f_args := []; f_local_vars := []; f_code := ∅; f_init := "" |}.
-Instance state_inhabited : Inhabited state := populate {| st_heap := inhabitant; st_allocs := inhabitant; st_fntbl := inhabitant; |}.
+Instance function_inhabited : Inhabited function :=
+  populate {| f_args := []; f_local_vars := []; f_code := ∅; f_init := "" |}.
+Instance heap_state_inhabited : Inhabited heap_state :=
+  populate {| hs_heap := inhabitant; hs_allocs := inhabitant; |}.
+Instance state_inhabited : Inhabited state :=
+  populate {| st_heap := inhabitant; st_fntbl := inhabitant; |}.
 
 Canonical Structure mbyteO := leibnizO mbyte.
 Canonical Structure functionO := leibnizO function.
@@ -1341,9 +1133,3 @@ Canonical Structure layoutO := leibnizO layout.
 Canonical Structure valO := leibnizO val.
 Canonical Structure exprO := leibnizO expr.
 Canonical Structure allocationO := leibnizO allocation.
-
-(*** Tests *)
-
-Example simpl_subst :
-  subst_stmt ([("y", [MPoison; MPoison]); ("x", [MPoison])]) (Return (BinOp AddOp PtrOp PtrOp (Var "x") (Var "y"))) = Return (BinOp AddOp PtrOp PtrOp (Val [MPoison]) (Val [MPoison; MPoison])).
-Proof. simpl. done. Abort.
