theories/lang/byte.v
@@ -1,0 +1,25 @@
+From refinedc.lang Require Import base.
+Open Scope Z_scope.
+
+(** Representation of a standard (8-bit) byte. *)
+
+Definition bits_per_byte : Z := 8.
+
+Definition byte_modulus : Z :=
+  Eval cbv in 2 ^ bits_per_byte.
+
+Record byte :=
+  Byte {
+    byte_val : Z;
+    byte_constr : -1 < byte_val < byte_modulus;
+  }.
+
+Program Definition byte0 : byte := {| byte_val := 0; |}.
+Next Obligation. done. Qed.
+
+Instance byte_eq_dec : EqDecision byte.
+Proof.
+  move => [b1 H1] [b2 H2]. destruct (decide (b1 = b2)) as [->|].
+  - left. assert (H1 = H2) as ->; [|done]. apply proof_irrel.
+  - right. naive_solver.
+Qed.
