theories/lang/int_type.v
@@ -1,0 +1,125 @@
+From refinedc.lang Require Import base byte layout.
+Open Scope Z_scope.
+
+(** Representation of an integer type (size and signedness). *)
+
+Definition signed := bool.
+
+Record int_type :=
+  IntType {
+    it_byte_size_log : nat;
+    it_signed : signed;
+  }.
+
+Definition bytes_per_int (it : int_type) : nat :=
+  2 ^ it.(it_byte_size_log).
+
+Definition bits_per_int (it : int_type) : Z :=
+  bytes_per_int it * bits_per_byte.
+
+Definition int_modulus (it : int_type) : Z :=
+  2 ^ bits_per_int it.
+
+Definition int_half_modulus (it : int_type) : Z :=
+  2 ^ (bits_per_int it - 1).
+
+(* Minimal representable integer. *)
+Definition min_int (it : int_type) : Z :=
+  if it.(it_signed) then - int_half_modulus it else 0.
+
+(* Maximal representable integer. *)
+Definition max_int (it : int_type) : Z :=
+  (if it.(it_signed) then int_half_modulus it else int_modulus it) - 1.
+
+Global Instance int_elem_of_it : ElemOf Z int_type :=
+  λ z it, min_int it ≤ z ≤ max_int it.
+
+Definition it_layout (it : int_type) :=
+  Layout (bytes_per_int it) it.(it_byte_size_log).
+
+Definition i8  := IntType 0 true.
+Definition u8  := IntType 0 false.
+Definition i16 := IntType 1 true.
+Definition u16 := IntType 1 false.
+Definition i32 := IntType 2 true.
+Definition u32 := IntType 2 false.
+Definition i64 := IntType 3 true.
+Definition u64 := IntType 3 false.
+
+(* hardcoding 64bit pointers for now *)
+Definition bytes_per_addr_log : nat := 3%nat.
+Definition bytes_per_addr : nat := (2 ^ bytes_per_addr_log)%nat.
+
+Definition intptr_t  := IntType bytes_per_addr_log true.
+Definition uintptr_t := IntType bytes_per_addr_log false.
+
+Definition size_t  := uintptr_t.
+Definition ssize_t := intptr_t.
+Definition bool_it := u8.
+
+(*** Lemmas about [int_type] *)
+
+Lemma bytes_per_int_gt_0 it : bytes_per_int it > 0.
+Proof.
+  rewrite /bytes_per_int. move: it => [log ?] /=.
+  rewrite Z2Nat_inj_pow. assert (0 < 2%nat ^ log); last lia.
+  apply Z.pow_pos_nonneg; lia.
+Qed.
+
+Lemma bits_per_int_gt_0 it : bits_per_int it > 0.
+Proof.
+  rewrite /bits_per_int /bits_per_byte.
+  suff : (bytes_per_int it > 0) by lia.
+  by apply: bytes_per_int_gt_0.
+Qed.
+
+Lemma int_modulus_twice_half_modulus (it : int_type) :
+  int_modulus it = 2 * int_half_modulus it.
+Proof.
+  rewrite /int_modulus /int_half_modulus.
+  rewrite -[X in X * _]Z.pow_1_r -Z.pow_add_r; try f_equal; try lia.
+  rewrite /bits_per_int /bytes_per_int.
+  apply Z.le_add_le_sub_l. rewrite Z.add_0_r.
+  rewrite Z2Nat_inj_pow.
+  assert (0 < 2%nat ^ it_byte_size_log it * bits_per_byte); last lia.
+  apply Z.mul_pos_pos; last (rewrite /bits_per_byte; lia).
+  apply Z.pow_pos_nonneg; lia.
+Qed.
+
+Lemma it_in_range_mod n it:
+  n ∈ it → it_signed it = false →
+  n `mod` int_modulus it = n.
+Proof.
+  move => [??] ?. rewrite Z.mod_small //.
+  destruct it as [? []] => //. unfold min_int, max_int in *. simpl in *.
+  lia.
+Qed.
+
+Lemma min_int_le_0 (it : int_type) : min_int it ≤ 0.
+Proof.
+  have ? := bytes_per_int_gt_0 it. rewrite /min_int /int_half_modulus.
+  destruct (it_signed it) => //. trans (- 2 ^ 7) => //.
+  rewrite -Z.opp_le_mono. apply Z.pow_le_mono_r => //.
+  rewrite /bits_per_int /bits_per_byte. lia.
+Qed.
+
+Lemma max_int_ge_127 (it : int_type) : 127 ≤ max_int it.
+Proof.
+  have ? := bytes_per_int_gt_0 it.
+  rewrite /max_int /int_modulus /int_half_modulus.
+  rewrite /bits_per_int /bits_per_byte.
+  have ->: (127 = 2 ^ 7 - 1) by []. apply Z.sub_le_mono => //.
+  destruct (it_signed it); apply Z.pow_le_mono_r; lia.
+Qed.
+
+Lemma int_modulus_mod_in_range n it:
+  it_signed it = false →
+  (n `mod` int_modulus it) ∈ it.
+Proof.
+  move => ?.
+  have [|??]:= Z.mod_pos_bound n (int_modulus it). {
+    apply: Z.pow_pos_nonneg => //. rewrite /bits_per_int/bits_per_byte/=. lia.
+  }
+  destruct it as [? []] => //.
+  split; unfold min_int, max_int => /=; lia.
+Qed.
