theories/lang/layout.v
@@ -1,0 +1,117 @@
+From refinedc.lang Require Import base.
+Open Scope Z_scope.
+
+(** Representation of a type layout (byte size and alignment constraint). *)
+
+Record layout :=
+  Layout {
+    ly_size : nat;
+    ly_align_log : nat;
+  }.
+
+Definition sizeof   (ly : layout) : nat := ly.(ly_size).
+Definition ly_align (ly : layout) : nat := 2 ^ ly.(ly_align_log).
+
+Instance layout_dec_eq : EqDecision layout.
+Proof. solve_decision. Defined.
+
+Instance layout_inhabited : Inhabited layout :=
+  populate (Layout 0 0).
+
+Instance layout_countable : Countable layout.
+Proof.
+  refine (inj_countable'
+    (λ ly, (ly.(ly_size), ly.(ly_align_log)))
+    (λ '(sz, a), Layout sz a) _); by intros [].
+Qed.
+
+Instance layout_le : SqSubsetEq layout := λ ly1 ly2,
+  (ly1.(ly_size) ≤ ly2.(ly_size))%nat ∧
+  (ly1.(ly_align_log) ≤ ly2.(ly_align_log))%nat.
+
+Instance layout_le_po : PreOrder layout_le.
+Proof.
+  split => ?; rewrite /layout_le => *; repeat case_bool_decide => //; lia.
+Qed.
+
+Definition ly_offset (ly : layout) (n : nat) : layout := {|
+  ly_size := ly.(ly_size) - n;
+  (* Sadly we need to have the second argument to factor2 as we want
+  that if l is aligned to x, then l + n * x is aligned to x for all n
+  including 0. *)
+  ly_align_log := ly.(ly_align_log) `min` factor2 n ly.(ly_align_log)
+|}.
+
+Definition ly_set_size (ly : layout) (n : nat) : layout := {|
+  ly_size := n;
+  ly_align_log := ly.(ly_align_log)
+|}.
+
+Definition ly_mult (ly : layout) (n : nat) : layout := {|
+  ly_size := ly.(ly_size) * n;
+  ly_align_log := ly.(ly_align_log)
+|}.
+
+Definition ly_with_align (sz : nat) (align : nat) : layout := {|
+  ly_size := sz;
+  ly_align_log := factor2 align 0
+|}.
+
+Definition layout_wf (ly : layout) : Prop := (ly_align ly | ly.(ly_size)).
+
+Lemma layout_wf_mod (ly : layout) :
+  ly.(ly_size) `mod` ly_align ly = 0 → layout_wf ly.
+Proof.
+  move => ?. apply Z.mod_divide => //. have ->: 0 = O by [].
+  move => /Nat2Z.inj/Nat.pow_nonzero. lia.
+Qed.
+
+Class LayoutWf (ly : layout) : Prop := layout_wf_wf : layout_wf ly.
+
+(* Class required because the combinators of layout are made typeclass opaque
+   later, so TCEq does not work. *)
+Class LayoutEq (ly1 ly2 : layout) : Prop := layout_eq : ly1 = ly2.
+
+Arguments ly_size : simpl never.
+Arguments sizeof _ /.
+Arguments ly_align : simpl never.
+
+Typeclasses Opaque layout_le ly_offset ly_set_size ly_mult ly_with_align.
+
+Hint Extern 0 (LayoutWf _) => refine (layout_wf_mod _ _); done : typeclass_instances.
+Hint Extern 0 (LayoutWf _) => unfold LayoutWf; done : typeclass_instances.
+Hint Extern 0 (LayoutEq _ _) => exact: eq_refl : typeclass_instances.
+
+(*** Lemmas about [layout] *)
+
+Lemma ly_align_log_ly_align_eq_iff ly1 ly2:
+  ly_align_log ly1 = ly_align_log ly2 ↔ ly_align ly1 = ly_align ly2.
+Proof. rewrite /ly_align. split; first naive_solver. move => /Nat.pow_inj_r. lia. Qed.
+
+Lemma ly_align_log_ly_align_le_iff ly1 ly2:
+  (ly_align_log ly1 ≤ ly_align_log ly2 ↔ ly_align ly1 ≤ ly_align ly2)%nat.
+Proof. rewrite /ly_align. apply: Nat.pow_le_mono_r_iff. lia. Qed.
+
+Lemma ly_size_ly_with_align m n :
+  ly_size (ly_with_align m n) = m.
+Proof. done. Qed.
+
+Lemma ly_align_ly_with_align m n :
+  ly_align (ly_with_align m n) = keep_factor2 n 1.
+Proof. rewrite /ly_with_align/keep_factor2/factor2. by destruct (factor2' n). Qed.
+
+Lemma ly_align_ly_offset ly n :
+  ly_align (ly_offset ly n) = (ly_align ly `min` keep_factor2 n (ly_align ly))%nat.
+Proof.
+  rewrite /ly_align/keep_factor2/=/factor2. destruct (factor2' n) as [n'|] => /=; last by rewrite !Nat.min_id.
+  destruct (decide (ly_align_log ly ≤ n'))%nat;[rewrite !min_l|rewrite !min_r]; try lia;
+    apply Nat.pow_le_mono_r; lia.
+Qed.
+
+Lemma ly_size_ly_set_size ly n:
+  ly_size (ly_set_size ly n) = n.
+Proof. done. Qed.
+
+Lemma ly_align_ly_set_size ly n:
+  ly_align (ly_set_size ly n) = ly_align ly.
+Proof. done. Qed.
